\documentclass[12pt]{article}
\usepackage{tikz}
\usepackage{amsmath}
\usepackage{amsthm}
\begin{document}
\title{STAT230 Assignment 2}
\author{Rin Meng \\ Student ID: 51940633}
\maketitle

\begin{enumerate}
	\item Given: $\sigma = 1.4$ cm, $\mu = 6$ cm, $x = 8$ cm.
		
		$Z = \frac{x - \mu}{\sigma} = \frac{8 - 6}{1.4} \simeq 1.43$ 
		\begin{enumerate}
			\item $P(Z \geq 1.43) = 1 - P(z \leq 1.43) = 1 - 0.9236 = 0.0764$
			\item $P(Z \leq 1.43) = 0.9236$
			\item In normal distribution, the Q1 and Q3 is given by:
			
			$$Q1 = \mu - 0.675 \sigma = 6 - 0.675(1.4) = 5.055$$
			
			$$Q3 = \mu + 0.675 \sigma = 6 + 0.675(1.4) = 6.945$$
			
			Therefore,
			
			$$IQR = Q3 - Q1 = 6.945 - 5.055 = 1.89$$
			
		\end{enumerate}
	\item Given: 
		\begin{itemize}
			\item Acceptance rate $= 1 - 0.04 - 0.10 = 0.86$
			\item Infimum (lower bound): $1 - 0.04 = 0.96 = P(Z \leq 1.75) \Rightarrow Z_{3.6mm} = -1.75 = \frac{3.6 - \mu}{\sigma}$
			\item Supremum (upper bound): $1 - 0.10 = 0.90 = P(Z \leq 1.28) \Rightarrow Z_{4.8mm} = 1.28 = \frac{4.8 - \mu}{\sigma}$
		\end{itemize}
		
		Solving for $\sigma$:
			$$\mu -1.75\sigma = 3.6$$
			$$\mu + 1.28\sigma = 4.8$$
			$$3.6 + 1.75 \sigma = \mu = 4.8 - 1.28 \sigma$$
			$$1.75 \sigma + 1.28 \sigma = 4.8 - 3.6$$
			$$3.03\sigma = 1.2$$
			$$\sigma = \frac{1.2}{3.03} \simeq 0.40$$
		Solving for $\mu$:
			$$\mu = 3.6 + 1.75(0.40)  \simeq 4.3$$
	\item Given: $f(t) = Ce^{-t/3}$
		\begin{enumerate}
			\item $F(t) = $
			 	$$\int_{0}^{\infty} Ce^{-t/3}dt = 1$$
				$$C\int_{0}^{\infty} e^{-t/3}dt = 1$$
				Use u-substitution: $u = -\frac{t}{3} \Rightarrow du = -\frac{1}{3}dt \Rightarrow dt = -3du$
				$$C\int_{0}^{\infty} e^{u}(-3 du) = 1$$
				$$-3C(e^{u})\vert_{0}^{\infty} = 1$$
				Substitute $-\frac{t}{3} = u$
				$$-3C(e^{-t/3})\vert_{0}^{\infty} = 1$$
				$$-3C(\lim\limits_{t \to \infty} e^{-\frac{t}{3}} -  e^{0}) = 1$$
				$$-3C(\lim\limits_{t \to \infty} \frac{1}{e^{t/3}} -  e^0) = 1$$
				$$-3C(0 - 1) = 1$$
				$$-3C(-1) = 1$$
				$$C = \frac{1}{3}$$
			\item Now that $C = \frac{1}{3}$,
				$$P(T > 5) = 1 - P(T < 5) = 1 - \frac{1}{3} \int_{0}^{5} e^{-t/3}dt$$
				$$P(T > 5) = 1 - \frac{1}{3} \int_{0}^{5} e^{-t/3}dt$$
				$$P(T > 5) = 1 - \frac{1}{3} \int_{0}^{5} e^{-t/3}dt$$
				Using the recent integrated integral, we can say that:
				$$P(T > 5) = 1 - \frac{1}{3} (-3e^{-t/3})\vert_{0}^{5}dt$$
				$$P(T > 5) = 1 + (e^{-5/3} - e^{0/3})$$
				$$P(T > 5) = 1 + (\frac{1}{e^{5/3}} - 1)$$
				$$P(T > 5) = 1 - 0.811 = 0.19$$
			\item Given that $C = \frac{1}{3}$ and $f(t) = Ce^{-t/3}$ then, 
			$$E[X] = \int_{-\infty}^{\infty} xf(x)dx = \int_{-\infty}^{\infty} \frac{1}{3}e^{-x/3}xdx$$
			$$E[X] = \int_{0}^{1} \frac{1}{3}e^{-x/3}xdx$$
			$$= \frac{1}{3}\int_{0}^{1} xe^{-x/3}dx$$
			Now solving for:
			$$\int xe^{-x/3}dx$$
			Substitute $u = -\frac{x}{3}, x = -3u \Rightarrow du = -\frac{1}{3}dx \Rightarrow dx = -3du$
			$$\int (-3u)e^{u}(-3du)$$
			$$= 9\int ue^{u}du$$ 
			Using integration by parts, $\int fg' = fg - \int f'g$
			
			$f = u$, $g' = e^u du$, $f' = du$, $g = e^u$
			$$\int ue^{u}du = ue^u - \int e^u du$$
			$$\int ue^{u}du = ue^u - e^u$$
			$$9 \int ue^{u}du = 9ue^u - 9e^u$$
			Substitute $-\frac{x}{3} = u$
			$$\frac{1}{3}\int_{0}^{1} e^{-x/3}xdx = \frac{1}{3} (-3xe^{-x/3} - 9e^{-x/3})\vert_{0}^{1}$$
			$$= \frac{1}{3}(-3xe^{-x/3} - 9e^{-x/3})\vert_{0}^{1}$$
			$$= -e^{-x/3}(x + 3)\vert_{0}^{1}$$
			$$= -e^{-1/3}(1 + 3) - (-e^{-0/3}(0 + 3))$$
			$$= -e^{-1/3}(4) - (-1(0 + 3))$$
			$$= -4e^{-1/3} - (-3)$$
			$$= -4e^{-1/3} + 3$$
			$$E[X] \simeq 0.134$$
		\end{enumerate}
		
		\item Given: Sample size: 500, population in favor of incumbent: 0.46
			\begin{enumerate}
				\item Since this is a Binomial Distribution, we have

				$P(X \geq 250) = 1 - P(X < 250)$
				
				$\mu = np = 500 \times 0.46 = 230$
				
				$\sigma = \sqrt{np(1-p)} = \sqrt{230(1-0.46)} \simeq 11.14$
				$$Z = \frac{x - \mu}{\sigma} = \frac{249.5 - 230}{11.14} = 1.75$$
				where x is adjusted for continuity correction, then we have:
				$$P(Z \geq 1.75) = 1 - P(Z < 1.75) = 1 - 0.9599 \simeq 0.04$$
				
				\item Given: sample $n = 50$. Using Poisson Approximation, the average success rate is $\lambda = np = 50(0.46) = 23$. So, it is true that
				$$P(X = x) = e^{-\lambda} \frac{\lambda^x}{x!} = e^{-23} \cdot \frac{23^{25}}{25!} = 0.073$$
				
				
				
				
				
			\end{enumerate}
			
		\item Given that: $f(x) = 2x$, $Y = g(x) = \frac{1}{1 + x}$
			
			Then it is true that:
			$$E[Y] = E[g(x)] = \int_{-\infty}^{\infty} g(x)f(x)dx$$
			$$\int_{0}^{1} \frac{2x}{1 + x}dx$$
			Solving by u-substitution: $u = 1 + x \Rightarrow x = u - 1 \Rightarrow du = dx$
			Supremum $= u = 1 + 1$, infimum $= u = 1 + 0$
			$$= \int_{1}^{2} \frac{2(u-1)}{u}du$$
			$$= \int_{1}^{2} \frac{2u-2}{u}du$$
			$$= \int_{1}^{2} 2 - \frac{2}{u}du$$
			$$= 2(u - ln(|u|)\vert_{1}^{2}du$$
			$$= 2(2 - ln(2)) - 2(1 - ln(1) = 2(1.31) - 2(1 - 0)$$
			$$E[Y] = 2.62 - 2 = 0.62$$
\end{enumerate}

End of Assignment 2.

\end{document}
